done Ch09

LeanConcreteSemantics/Ch07IMP.lean
@@ -1,7 +1,8 @@
-
 import LeanConcreteSemantics.Ch03ImpExpr
+import LeanConcreteSemantics.Ch02Proving
 
 set_option pp.fieldNotation false
+set_option pp.proofs true
 
 open section_3_1
 open section_3_1.Aexp
@@ -213,19 +214,340 @@ theorem if_c_c : ∀ { b c }, (IF b THEN c ELSE c) ≃ c := by
      .case false => apply BigStep.IfFalse <;> assumption
      .case true  => apply BigStep.IfTrue  <;> assumption
 
-theorem boo : ∀ {b c c' s t},
+theorem lem_7_6 : ∀ {b c c' s t},
   (⟨ WHILE b DO c END , s ⟩ ==> t) ->
   c ≃ c' ->
   (⟨ WHILE b DO c' END, s ⟩ ==> t) := by
-  intros b c c' s t cst cc
-  induction cst -- nasty error: index in target's type is not a variable (consider using the `cases` tactic instead)
+   intros b c c' s t cst c_eq_c'
+   generalize h : (WHILE b DO c END) = x at cst   --- this is ANF / Nico's tip
+   induction cst <;> simp_all []
+   . case WhileFalse =>
+      constructor
+      assumption
+   . case WhileTrue =>
+      constructor <;> try assumption
+      simp_all [equiv_com]    --- this is a bit of magic
 
-  -- cases hb : bval b s
-  -- . case false =>
-  --   cases cst
-  --   . case WhileFalse => apply BigStep.WhileFalse <;> assumption
-  --   . case WhileTrue  => simp_all []
-  -- . case true =>
-  --   cases cst
-  --   . case WhileFalse => simp_all []
-  --   . case WhileTrue s1 _ c_s_s1 w_c_s1_t => sorry
+theorem equiv_symm : ∀ {c c'}, c ≃ c' -> c' ≃ c := by
+  simp_all [equiv_com]
+
+theorem equiv_refl : ∀ {c}, c ≃ c := by
+  simp_all [equiv_com]
+
+theorem equiv_trans : ∀ {c1 c2 c3}, c1 ≃ c2 -> c2 ≃ c3 -> c1 ≃ c3 := by
+  simp_all [equiv_com]
+
+theorem lem_7_5 : ∀ {b c c'},
+  c ≃ c' ->
+  (WHILE b DO c END) ≃ (WHILE b DO c' END) := by
+  intros b c c' c_eq_c'
+  simp_all [equiv_com]
+  intros st st'
+  apply Iff.intro
+  . case mp =>
+      intros wc
+      apply lem_7_6
+      assumption
+      assumption
+  . case mpr =>
+      intros wc
+      apply lem_7_6
+      assumption
+      apply equiv_symm
+      assumption
+
+theorem bigstep_deterministic : ∀ {c s t1 t2}, (⟨ c, s ⟩ ==> t1) -> (⟨ c, s ⟩ ==> t2) -> t1 = t2 := by
+  intros c s t1 t2 s_to_t1 s_to_t2
+  induction s_to_t1 generalizing t2 <;> cases s_to_t2 <;> try simp_all []
+  case Seq.Seq =>
+    rename_i c1 c2 st1 st2 st3 _ _ ih1 ih2 _ bob _
+    apply ih2
+    have fact := ih1 bob
+    simp_all []
+  case WhileTrue.WhileTrue =>
+    rename_i b c st st' st'' _ _ ih1 ih2 _ _ bob _
+    apply ih2
+    have fact := ih1 bob
+    simp_all []
+  case IfTrue.IfTrue =>
+    rename_i b c1 c2 _ _ _ ih _ _
+    apply ih
+    simp_all []
+  case IfFalse.IfFalse =>
+    rename_i b c1 c2 _ _ _ ih _ _
+    apply ih
+    simp_all []
+
+inductive Step : (Com × State) -> (Com × State) -> Prop where
+   | Assign : ∀ {x a s},
+                Step (x <~ a, s) (Skip, s [x := aval a s])
+   | Seq1   : ∀ {c s},
+                Step ((Skip ;; c), s) (c, s)
+   | Seq2   : ∀ {c1 c1' c2 s s'},
+                Step (c1, s) (c1', s') ->
+                Step ((c1 ;; c2) , s) ((c1' ;; c2), s')
+   | IfTrue : ∀ {b c1 c2 s},
+                bval b s == true ->
+                Step (IF b THEN c1 ELSE c2, s) (c1, s)
+   | IfFalse : ∀ {b c1 c2 s},
+                bval b s == false ->
+                Step (IF b THEN c1 ELSE c2, s) (c2, s)
+   | While   : ∀ { b c s },
+                Step (Com.While b c, s) (Com.If b (c ;; (Com.While b c)) Skip, s)
+
+open section_4_5 (star)
+
+abbrev Steps := star Step
+
+def com_xz_yx := x <~ Var z ;; y <~ Var x
+
+def st := st0 ["x" := 3] [ "y" := 7 ] [ "z" := 5 ]
+
+theorem smallstep_deterministic : ∀ {cs cs1 cs2}, (Step cs cs1) -> (Step cs cs2) -> cs1 = cs2 := by
+  intros cs cs1 cs2 step1 step2
+  induction step1 generalizing cs2 <;> cases step2 <;> simp_all []
+  case Seq2.Seq1  _ _ _ _ b _ => cases b
+  case Seq1.Seq2  _ _ _ _  b  => cases b
+  case Seq2.Seq2 =>
+    rename_i c11 c11' _ _ _ _ ih _ _ step_c11
+    have fact := ih step_c11
+    simp_all []
+
+theorem steps_skip : ∀ {st cs}, Steps (Skip, st) cs -> cs = (Skip, st) := by
+  intros st cs steps
+  cases steps
+  . case refl => simp_all []
+  . case step _ ih _ => cases ih
+
+theorem seq_steps : ∀ {c1 c1' c2 s s'},
+  Steps (c1, s) (c1', s') ->
+  Steps (c1;;c2, s) (c1';;c2, s')
+  := by
+  intros c1 c1' c2 s s' steps_c1_c1'
+  generalize h1 : (c1, s)   = c1s  at steps_c1_c1'
+  generalize h2 : (c1', s') = c1s' at steps_c1_c1'
+  induction steps_c1_c1' generalizing c1 c1' c2 s s'
+  case refl =>
+    rename_i a
+    cases h1
+    simp_all []
+    apply star.refl
+  case step  =>
+    cases h1
+    cases h2
+    rename_i c1s'' step_c1_hd _ ih
+    apply star.step
+    constructor
+    apply step_c1_hd
+    apply ih
+    simp_all []
+    simp_all []
+
+
+theorem skip_steps : ∀ {c st1 st2},
+  star Step (c, st1) (Skip, st2) ->
+  star Step (Skip;;c , st1) (Skip, st2) := by
+  intros
+  apply star.step
+  constructor
+  assumption
+
+---------------------------------------------------------------------------------
+@[simp] theorem BigStep_skip_Iff : ∀ {s t}, (⟨ Skip, s ⟩ ==> t) <-> (s = t) := by
+  intros s t
+  apply Iff.intro
+  . case mp =>
+      intro h
+      cases h
+      simp_all []
+  . case mpr =>
+      intro s_eq_t
+      simp_all []
+      constructor
+
+@[simp] theorem BigStep_assign_Iff: ∀ {x a s t}, (⟨ x <~ a, s ⟩ ==> t) <-> (t = (s[x := aval a s])) := by
+  intros x a s t
+  apply Iff.intro
+  . case mp =>
+      intro h
+      cases h
+      simp_all []
+  . case mpr =>
+      intro h
+      simp_all []
+      constructor
+
+@[simp] theorem BigStep_seq_Iff: ∀ {c1 c2 s t}, (⟨ c1 ;; c2, s ⟩ ==> t) <-> (∃ s', (⟨ c1, s ⟩ ==> s') ∧ (⟨ c2, s' ⟩ ==> t)) := by
+  intros c1 c2 s t
+  apply Iff.intro
+  . case mp =>
+    intros h
+    cases h
+    apply Exists.intro
+    apply And.intro
+    assumption
+    assumption
+  . case mpr =>
+    intros h
+    cases h
+    rename_i s' h12
+    cases h12
+    constructor
+    assumption
+    assumption
+
+@[simp] theorem BigStep_if_Iff: ∀ {b c1 c2 s t}, (⟨ IF b THEN c1 ELSE c2 , s ⟩ ==> t) <-> ((bval b s = true ∧ (⟨ c1, s ⟩ ==> t)) ∨ (bval b s = false ∧ (⟨ c2, s ⟩ ==> t))) := by
+  intros b c1 c2 s t
+  apply Iff.intro
+  . case mp =>
+    intro h
+    cases h
+    . case IfTrue =>
+      apply Or.inl
+      apply And.intro
+      assumption
+      assumption
+    . case IfFalse =>
+      apply Or.inr
+      apply And.intro
+      assumption
+      assumption
+  . case mpr =>
+    intro h
+    cases h
+    . case inl h =>
+      cases h
+      apply BigStep.IfTrue
+      assumption
+      assumption
+    . case inr h =>
+      cases h
+      apply BigStep.IfFalse
+      assumption
+      assumption
+
+#check BigStep.WhileTrue
+
+theorem bigstep_implies_smallstep : ∀ {c s t}, (⟨ c, s ⟩ ==> t) -> Steps (c, s) (Skip, t) := by
+  intros c s t bs
+  induction bs
+  . case Skip => constructor
+  . case Assign s x a => apply star.step
+                         constructor
+                         apply star.refl
+  . case Seq c1 c2 st1 st2 st3 _ _ sc1 sc2 =>
+      apply section_4_5.star_trans
+      apply seq_steps
+      apply sc1
+      apply star.step
+      apply Step.Seq1
+      apply sc2
+  . case IfTrue =>
+      apply star.step
+      apply Step.IfTrue
+      simp_all []
+      assumption
+  . case IfFalse =>
+      apply star.step
+      apply Step.IfFalse
+      simp_all []
+      assumption
+  . case WhileFalse b c st b_false =>
+      apply star.step
+      constructor
+      apply section_4_5.star_one
+      constructor
+      simp_all []
+  . case WhileTrue =>
+      rename_i b c st st1 st2 _ _ _ c_steps ih
+      apply star.step
+      constructor
+      apply star.step
+      constructor <;> simp_all []
+      apply section_4_5.star_trans
+      apply seq_steps c_steps
+      apply skip_steps
+      assumption
+
+theorem step_case : ∀ {c c' s s' t},  Step (c, s) (c', s') -> (⟨ c', s' ⟩ ==> t) -> (⟨ c, s ⟩ ==> t) := by
+  intros c c' s s' t step1 bigstep
+  generalize h : (c, s) = cs at step1 --- this is ANF / Nico's tip
+  generalize h : (c', s') = cs' at step1 --- this is ANF / Nico's tip
+  induction step1 generalizing c c' s s' t
+  . case Assign x a s hyp  =>
+      cases h
+      cases hyp
+      simp_all []
+  . case Seq1 c s hyp =>
+      cases h
+      cases hyp
+      constructor
+      constructor
+      assumption
+  . case Seq2 c1 c1' c2 s s' _hyp step_c1 ih =>
+      cases ih
+      cases h
+      cases bigstep
+      rename_i st2 c1'_s'_st2' c2_st2
+      constructor
+      apply step_c1
+      apply c1'_s'_st2'
+      simp_all []
+      simp_all []
+      assumption
+  . case IfTrue b c1 c2 s hyp hh  =>
+      cases h
+      cases hh
+      constructor
+      simp_all []
+      assumption
+  . case IfFalse b c1 c2 s hyp hh =>
+      cases h
+      cases hh
+      apply BigStep.IfFalse
+      simp_all []
+      assumption
+  . case While b c s hh =>
+      cases h
+      cases hh
+      generalize hyp : bval b s = bv
+      cases bv
+      -- bv = false
+      cases bigstep
+      simp_all []
+      simp_all []
+      apply BigStep.WhileFalse
+      assumption
+      -- bv = true
+      cases bigstep
+      simp_all []
+      rename_i h_bv h_c_w
+      cases h_c_w
+      rename_i s' hh
+      cases hh
+      apply BigStep.WhileTrue
+      assumption
+      assumption
+      assumption
+      simp_all []
+
+
+
+
+theorem smallstep_implies_bigstep : ∀ {c s t}, Steps (c, s) (Skip, t) -> (⟨ c, s ⟩ ==> t)  := by
+  intros c s t steps
+  generalize h : (c, s)    = x at steps --- this is ANF / Nico's tip
+  generalize h : (Skip, t) = y at steps --- this is ANF / Nico's tip
+  induction steps generalizing c s t
+  . case refl h1 h2 =>
+      cases h2
+      cases h
+      constructor
+  . case step cs cs1 skip_t step_head step_tail ih h7 =>
+      cases h7
+      cases h
+      apply step_case
+      apply step_head
+      apply ih
+      simp_all []
+      simp_all []
